coq-osiris/theories/program_logic/pure/unary_fun_spec.v
@@ -1,0 +1,109 @@
+From osiris Require Import base.
+From osiris.lang Require Import lang.
+From osiris.semantics Require Import semantics.
+From osiris.program_logic Require Import pure_rules.
+From osiris.program_logic Require Import pure.toplevel_rules.
+From osiris.program_logic Require Import pure.fun_spec.
+
+From stdpp Require Import well_founded.
+
+(** This file is to be used as motivation for the [Spec] predicate.
+    As an example, we define [Spec'] as a way to specify unary functions.
+
+    For the actual treatment of function specifications, see [fun_spec.v] *)
+
+(* -------------------------------------------------------------------------- *)
+
+(* [call_spec] is the type of specifications over function calls. It
+   depends on two arguments: the argument of the function call, and the
+   computation resulting from calling the function on that argument. *)
+
+Local Definition call_spec' {X : Type} := X -> microvx -> Prop.
+
+(* [Spec' c P] states that given a closure [c], the specification [P]
+   holds for any call of [c] on an argument. *)
+
+Local Definition Spec' `{Encode X} (c : val) (P : call_spec') :=
+  ∀ (x : X), P x (fun_spec.call c #x).
+
+(* -------------------------------------------------------------------------- *)
+
+(* Consider for example the specification of a function [sort]:
+   [ Spec' sort (λ l m, pure m (λ l', Sorted l' ∧ l' ≡ l) ⊥) ] *)
+
+(* Example of a reasoning rule, for the creation of a [Spec' c P]. *)
+
+Local Lemma pure_eval_anon' `{Encode X} (P : call_spec') η (xvar : var) e ζ :
+  (∀ (x : X),
+      P x (eval ((xvar, #x) :: η) e)) ->
+  pure (eval η (EAnonFun (AnonFun xvar e))) (λ c, Spec' c P) ζ.
+Proof. by intros; simpl_eval; eapply pure_ret. Qed.
+
+
+(* [pure_call_spec'] illustrates how we may want to use a [Spec c P]
+   specification. *)
+
+Local Lemma pure_call_spec' `{Encode X, Encode Y} (P : X -> microvx -> Prop) c v (φ : Y -> Prop) ζ :
+  Spec' c P ->
+  (∀ m, P v m -> pure m φ ζ) ->
+  pure (eval.call c #v) φ ζ.
+Proof.
+  intros HSpec Hmon. eapply pure_call_equiv.
+  apply Hmon. apply HSpec.
+Qed.
+
+(* -------------------------------------------------------------------------- *)
+
+(* [pure_eval_letrec'] allows us to prove that the body [e] of a letrec
+   expression satisfies a specification given by [P].
+
+   In a first subgoal, we prove that any function call satisfies [P],
+   under the assumption that calls to smaller arguments (according to
+   [R]) are well-behaved.
+   In the second subgoal, we prove [e2] while abstracting over [e]. *)
+
+Local Lemma pure_eval_letrec' `{Encode X, Encode Y}
+  (P : call_spec') (R : X -> X -> Prop) η f (x : var) e
+  e2 (φ : Y -> Prop) ζ :
+  (* Show that the relation on which arguments are decreasing is well-founded. *)
+  wf R ->
+  (* Show the specification [P] holds over a call to any argument
+     [arg], under the assumption that [P] holds to a call over any
+     argument [yval] smaller than [arg]. *)
+  (∀ c (arg : X),
+      Spec' c (λ yval m, R yval arg -> P yval m) ->
+      P arg (eval ((x, #arg) :: (f, c) :: η) e)) ->
+  (* Continue with [f] bound to [c], and [c] specified by [P]. *)
+  (∀ c, Spec' c P -> pure (eval ((f, c) :: η) e2) φ ζ) ->
+  (* When facing an expression of the form [let rec f x = e in e2]. *)
+  pure (eval η (ELetRec [RecBinding f (AnonFun x e)] e2)) φ ζ.
+Proof.
+  intros Hwf Hmkspec He2. simpl_eval. eapply He2.
+  unfold Spec'. intros v.
+  induction v as [v IH] using (well_founded_induction Hwf); intros.
+  simpl; rewrite String.eqb_refl; simpl.
+  eapply Hmkspec. intros y. intros HR. by apply IH.
+Qed.
+
+(* [structs_letrec'] mirrors [pure_eval_letrec'],
+   dealing with top-level let-recs [ILetRec] instead of
+   inline let-recs [ELetRec]. *)
+
+Local Lemma structs_letrec' `{Encode X} (R : X -> X -> Prop) η δ f (x : var) e
+  (P : X -> microvx -> Prop)
+  sitems φ :
+  wf R ->
+  (∀ c v',
+      Spec' c (λ v m, R v v' -> P v m) ->
+      P v' (eval ((x, #v') :: (f, c) :: η) e)) ->
+  (∀ c, Spec' c P ->
+       struct_items ((f, c) :: η, (f, c) :: δ) sitems φ) ->
+  struct_items (η, δ) (ILetRec [RecBinding f (AnonFun x e)] :: sitems) φ.
+Proof.
+  intros Hwf Hmkspec He2.
+  unfold struct_items; simpl_eval_sitems.
+  eapply He2. intros v.
+  induction v as [v IH] using (well_founded_induction Hwf); intros.
+  simpl; rewrite String.eqb_refl; simpl.
+  by eapply Hmkspec.
+Qed.
